Framework.v
@@ -1,5 +1,6 @@
 From vchez Require Export Definitions.
 From TLC Require Import LibLN.
+From TLC Require Import LibReflect.
 From Coq Require Export List.
 
 Hint Constructors s_term : core.
@@ -30,6 +31,25 @@ Hint Resolve s_term_abs_to_body
              t_term_abs_to_body 
              s_body_to_term_abs
              t_body_to_term_abs.
+
+Lemma s_subst_id : forall t x u,
+  x \notin s_fv t -> s_subst x u t = t.
+Proof.
+  intros. induction t; simpls; f_equal~; eauto.
+  induction ts; simpls. reflexivity.
+  - apply notin_union in H. destruct H. rewrite IHts.
+    + f_equal~. admit.
+    + apply H0.
+  - admit.
+  - unfold notin in H. rewrite in_singleton in H.   
+    + rewrite var_compare_eq. rewrite if_isTrue.
+      unfold not in H. admit.
+Admitted.
+
+
+     
+    
+    
 
 (*
 To Prove:
